Commit

Compiler/CompilerProof.v
@@ -1,6 +1,6 @@
 Require Import LibTactics assertion_lemmas GPUCSL TypedTerm Monad
-        Host DepList CUDALib CSLLemma CSLTactics Compiler Correctness CodeGenM.
-
+        Host DepList CUDALib CSLLemma CSLTactics CodeGen Compiler mkMap mkReduce
+        Correctness CodeGenM SeqCompilerProof.
 
 Definition main_spec GA :=
   let ps := gen_params GA in
@@ -9,6 +9,74 @@ Definition main_spec GA :=
      fs_tri := (All (apEnv : APtrEnv GA) (aeEnv : AEvalEnv GA),
                 FDbl (kernelInv (remove_typeinfo ps) apEnv aeEnv Emp True nil 1)
                      ((fun _ _ => True) ** (kernelInv (remove_typeinfo ps) apEnv aeEnv Emp True nil 1))) |}.
+
+Lemma compile_map_ok GA dom cod ntrd nblk
+      (avenv : AVarEnv GA) (apenv : APtrEnv GA) (aeenv : AEvalEnv GA)
+      (f : Skel.Func GA (Skel.Fun1 dom cod))
+      (arr : Skel.AE GA dom) (result : Skel.aTypDenote cod)
+      xs fns Gp :
+  Skel.skelDenote GA cod (Skel.Map GA dom cod f arr) aeenv = Some result
+  -> ST_ok (preST xs fns (kernelInv avenv apenv aeenv Emp True nil 1) Gp)
+           (compile_map ntrd nblk avenv f arr)
+           (fun res => postST xs fns (kernelInv avenv apenv aeenv Emp True nil 1)
+                              (Ex ps len, kernelInv avenv apenv aeenv
+                                                    (arrays (val2gl ps) (arr2CUDA result) 1%Qc)
+                                                    True
+                                                    (fst res |-> len :: snd res |=> ps) 1%Qc) Gp nil).
+Proof.
+  intros Heval.
+  unfold compile_map; simpl.
+  eapply rule_backward.
+  evar (ftri : FTri).
+  eapply rule_bind.
+  { applys (>>rule_gen_kernel).
+    skip. skip.
+    intros.
+    Definition interp_program_n_simp p fs n :=
+      interp_ftri (fs_tri fs) (fun P Q => forall ntrd nblk, CSLg_n ntrd nblk P p Q n).
+    Definition interp_program M G p fs :=
+      with_ctx M G (fun n => interp_program_n_simp p fs n).
+
+    Lemma interp_fd_kfun M G k fs :
+      interp_program M G (body_of k) fs -> interp_kfun M G k fs.
+    Proof.
+      unfold interp_program, interp_kfun, with_ctx; intros Hsat n Hctx.
+      forwards* Hsat': Hsat.
+      unfold interp_program_n_simp, interp_kfun_n_simp, CSLkfun_n_simp, CSLg_n in *.
+      destruct fs as [? ? ftri]; simpl in *.
+      destruct k; simpl in *.
+      induction ftri; simpl in *; eauto.
+    Qed.
+    Lemma mkMap_ok M G GA dom cod arr_c f_c pars tag :
+      interp_kfun M G (mkMap GA dom cod arr_c f_c)
+                     (FS pars tag
+                         (All ntrd nblk avar_env aptr_env aeval_env arr f result eval_map_ok outp outs,
+                          FDbl (kernelInv avar_env aptr_env aeval_env (arrays (val2gl outp) outs 1)
+                                          True
+                                          ("nblk" |-> Zn nblk :: "ntrd" |-> Zn ntrd :: inp_len_name |-> G.Zn
+                                                  (Datatypes.length (mkMap.arr_res GA aeval_env dom cod arr f result eval_map_ok)) :: mkMap.outArr cod |=> outp) 1)
+                               (kernelInv' aptr_env aeval_env (arrays (val2gl outp) (arr2CUDA result) 1) True 1))).
+        apply interp_fd_kfun.
+        unfold interp_program, interp_program_n_simp; simpl.
+        intros n Hctx ntrd nblk avar_env aptr_env aeval_env arr f result eval_map_ok outp outs.
+        introv. 
+
+        Lemma CSLg_CSLg_n ntrd nblk P p Q : CSLg ntrd nblk P p Q -> forall n, CSLg_n ntrd nblk P p Q n.
+        Proof. unfold CSLg, CSLg_n; eauto. Qed.
+        apply CSLg_CSLg_n.
+
+
+
+
+
+          
+
+        apply mkMap_prog_ok.
+
+    apply interp_fd_kfun.
+    unfold mkMap; simpl.
+
+
 
 Theorem compile_AS_ok GA ty ntrd nblk (p : Skel.AS GA ty) :
   let M := compile_prog ntrd nblk p in
